Finished LimitedStack and changed indentation to 4 spaces

LimitedStack.dfy
@@ -1,90 +1,91 @@
 // A LIFO queue (aka a stack) with limited capacity.
 class LimitedStack{
 
-      var capacity : int; // capacity, max number of elements allowed on the stack.
-      var arr : array?<int>; // contents of stack.
-      var top : int; // The index of the top of the stack, or -1 if the stack is empty
+    var capacity : int; // capacity, max number of elements allowed on the stack.
+    var arr : array?<int>; // contents of stack.
+    var top : int; // The index of the top of the stack, or -1 if the stack is empty
 
-      // This predicate express a class invariant: All objects of this calls should satisfy this.
-      predicate Valid()
-      reads this;
-      {
-          arr != null && capacity > 0 && capacity == arr.Length && top >= -1 && top < capacity
-      }
+    // This predicate express a class invariant: All objects of this calls should satisfy this.
+    predicate Valid()
+        reads this;
+    {
+        arr != null && 0 < capacity == arr.Length && top >= -1 && top < capacity
+    }
 
-      predicate Empty()
-      reads this;
-      {
-          top == -1
-      }
+    predicate Empty()
+        reads this;
+    {
+        top == -1
+    }
 
-      predicate Full()
-      reads this;
-      {
-          top == capacity - 1
-      }
+    predicate Full()
+        reads this;
+    {
+        top == capacity - 1
+    }
 
-      method Init(c : int)
-      modifies this;
-      requires c > 0;
+    method Init(c : int)
+        requires c > 0;
+        ensures Valid() && Empty() && !Full() && capacity == c;
+        ensures fresh(arr); // ensures arr is a newly created object.
 
-      ensures fresh(arr); // ensures arr is a newly created object.
-      ensures Valid();
-      ensures Empty();
-
-      {
+        modifies this;
+    {
         capacity := c;
         arr := new int[c];
         top := -1;
-      }
+    }
 
      
-      method isEmpty() returns (res : bool)
-      requires Empty();
-      {
-            res := true;
-      }
+    method isEmpty() returns (res : bool)
+        requires Empty();
+    {
+        res := true;
+    }
 
 
-      // Returns the top element of the stack, without removing it.
-      method Peek() returns (elem : int)
-      requires Valid();
-      requires !Empty();
-      {
-          elem := arr[top];
-      }
-
-      // Pushed an element to the top of a (non full) stack. 
-      method Push(elem : int)
-      requires Valid() && !Full();
-
-      ensures !Empty() && Valid();
-    
-      modifies this.arr, this`top;
-      {
-          top := top + 1;
-          arr[top] := elem;
-      }
-
-      // Pops the top element off the stack.
-      method Pop() returns (elem : int)
+    // Returns the top element of the stack, without removing it.
+    method Peek() returns (elem : int)
         requires Valid() && !Empty();
+        ensures elem == arr[top];
+    {
+        elem := arr[top];
+    }
 
-        ensures !Full() && Valid();
+    // Pushed an element to the top of a (non full) stack. 
+    method Push(elem : int)
+        requires Valid() && !Full();
+        ensures Valid() && !Empty();
+        ensures arr[top] == elem && old(top) + 1 == top;
+        ensures forall i :: 0 <= i < top ==> arr[i] == old(arr[i]);
+
+        modifies this.arr, this`top;
+    {
+        top := top + 1;
+        arr[top] := elem;
+    }
+
+    // Pops the top element off the stack.
+    method Pop() returns (elem : int)
+        requires Valid() && !Empty();
+        ensures Valid() && !Full();
+        ensures elem == arr[old(top)];
+        ensures top == old(top) - 1;
 
         modifies this`top;
-      {
-          elem := arr[top];
-          top := top-1;
-      }
+    {
+        elem := arr[top];
+        top := top - 1;
+    }
  
-      method Shift()
-      requires Valid() && !Empty();
-      ensures Valid();
-      ensures forall i : int :: 0 <= i < capacity - 1 ==> arr[i] == old(arr[i + 1]);
-      ensures top == old(top) - 1;
-      modifies this.arr, this`top;
-      {
+    method Shift()
+        requires Valid() && !Empty();
+        ensures Valid();
+        ensures forall i : int :: 0 <= i < capacity - 1 ==> arr[i] == old(arr[i + 1]);
+        ensures top == old(top) - 1;
+
+        modifies this.arr, this`top;
+    {
         var i : int := 0;
         while (i < capacity - 1 )
         invariant 0 <= i < capacity;
@@ -92,55 +93,60 @@ class LimitedStack{
         invariant forall j : int :: 0 <= j < i ==> arr[j] == old(arr[j + 1]);
         invariant forall j : int :: i <= j < capacity ==> arr[j] == old(arr[j]);
         {
-          arr[i] := arr[i + 1];
-          i := i + 1;
+            arr[i] := arr[i + 1];
+            i := i + 1;
         }
         top := top - 1;
-      }
+    }
 
-      //Push onto full stack, oldest element is discarded.
-      method Push2(elem : int)
-      requires Valid();
+    //Push onto full stack, oldest element is discarded.
+    method Push2(elem : int)
+        requires Valid();
+        ensures Valid() && !Empty();
+        ensures !old(Full()) ==> old(top) + 1 == top;
+        ensures old(Full()) ==> old(top) == top;
+        ensures arr[top] == elem;
+        ensures old(Full()) ==> (forall i :: 0 <= i < top ==> arr[i] == old(arr[i + 1]));
+        modifies this.arr, this`top;
 
-      modifies this.arr, this`top;
-      {
-            if(top == capacity-1) {
-                Shift();
-            }
-            top := top+1;
-            arr[top] := elem;
-      }
+        modifies this.arr, this`top;
+    {
+        if(top == capacity-1) {
+            Shift();
+        }
+        top := top+1;
+        arr[top] := elem;
+    }
 
 
 // When you are finished,  all the below assertions should be provable. 
 // Feel free to add extra ones as well.
-      method Main(){
-           var s := new LimitedStack;
-           s.Init(3);
+    method Main(){
+        var s := new LimitedStack;
+        s.Init(3);
 
-           assert s.Empty() && !s.Full(); 
+        assert s.Empty() && !s.Full(); 
 
-           s.Push(27);
-           assert !s.Empty();
+        s.Push(27);
+        assert !s.Empty();
 
-           var e := s.Pop();
-           assert e == 27;
+        var e := s.Pop();
+        assert e == 27;
 
-           s.Push(5);
-           s.Push(32);
-           s.Push(9);
-           assert s.Full();
+        s.Push(5);
+        s.Push(32);
+        s.Push(9);
+        assert s.Full();
 
-           var e2 := s.Pop();
-           assert e2 == 9 && !s.Full(); 
-           assert s.arr[0] == 5;
+        var e2 := s.Pop();
+        assert e2 == 9 && !s.Full(); 
+        assert s.arr[0] == 5;
 
-           s.Push(e2);
-           s.Push2(99);
+        s.Push(e2);
+        s.Push2(99);
 
-           var e3 := s.Peek();
-           assert e3 == 99;
-           assert s.arr[0] == 32;
-                     
-       }
+        var e3 := s.Peek();
+        assert e3 == 99;
+        assert s.arr[0] == 32;
+    }
 }
